rustexamples/test/borrow_test/27.rs
@@ -1,0 +1,8 @@
+fn return_bor_or_modify<'a>(x: &'a mut i32) -> &'a mut i32{
+    if *x > 3 {
+        let r : &mut i32 = &mut *x;
+        return r;
+    }
+    *x = 4;
+    return x;
+}
